src/Syntax.v
@@ -78,6 +78,11 @@ Coercion EExp : NonVal >-> Exp.
 Notation "` v" := (VVal v) (at level 11).
 Notation "° n" := (EExp n) (at level 11).
 
+Definition inf :=
+  ELetRec
+    [(0, °EApp (`VFunId (0, 0)) [])]
+    (EApp (`VFunId (0, 0)) []).
+
 (** Shorthands: *)
 Definition VEmptyMap : Val := VMap [].
 Definition VEmptyTuple : Val := VTuple [].
